towards plurality refine

theories/Compositional_Structures/Basic_Modules/Plurality_Module_Ref.thy
@@ -12,29 +12,38 @@ fun plurality_r :: "'a Electoral_Module_Ref" where
      {})"
 
 lemma datarefplurality:
-  assumes "A \<noteq>{}"
-  shows "(plurality_r A, plurality A) \<in> (br pa_to_pr (profile_a A)) \<rightarrow> 
+  shows "(plurality_r, plurality) \<in> Id \<rightarrow> (br pa_to_pr (profile_a A)) \<rightarrow> 
     Id"
   apply (refine_rcg)
-  using assms apply (auto simp add: 
-    refine_rel_defs) 
+  apply (auto simp add: 
+    refine_rel_defs win_count_array) 
   done
+  
+
+lemma plurality_r_sound:
+  shows "electoral_module_r plurality_r"
+  using datarefplurality plurality_sound
+  unfolding electoral_module_def electoral_module_r_def
+  apply safe
+  oops
+
 
 type_synonym 'a Electoral_Module_Ref_T = "'a set \<Rightarrow> 'a Profile_Array \<Rightarrow> 'a Result_Ref nres"
 
 definition initmap :: "'a set \<Rightarrow> 'a \<rightharpoonup> nat" where
   "initmap A = (SOME m. (\<forall>a\<in>A. ((m a) = Some (0::nat))))"
 
-
+definition "computewcinvar A p \<equiv> \<lambda>(i, wcmap).
+  \<forall>a\<in>A. the (wcmap a) = win_count_imp_code (array_shrink p i) a"
 
 definition computewcforcands :: "'a set \<Rightarrow> 'a Profile_Array \<Rightarrow> ('a \<rightharpoonup> nat) nres" where
-  "computewcforcands A p \<equiv> do {               
+  "computewcforcands A p \<equiv> do {
+    let wcmap = initmap A;               
     (i, wcmap) \<leftarrow> WHILET (\<lambda>(i, _). i < array_length p) (\<lambda>(i, wcmap). do {
       ASSERT (i < array_length p);
       let ballot = (p[[i]]);
-      let winner = (ballot[[0]]);
-      let wcmap = (if (wcmap winner = None) then wcmap (winner \<mapsto> 0)
-           else wcmap (winner \<mapsto> (the (wcmap winner) + 1)));
+      let wcmap = (if (array_length ballot > 0) then (
+        wcmap ((ballot[[0]]) \<mapsto> (the (wcmap (ballot[[0]]))) + 1)) else wcmap);
       let i = i + 1;
      RETURN (i, wcmap)
     })(0, Map.empty);
@@ -44,8 +53,10 @@ definition computewcforcands :: "'a set \<Rightarrow> 'a Profile_Array \<Rightar
 lemma wcmap_correc : assumes "profile_a A p"
   shows "computewcforcands A p \<le> SPEC (\<lambda> m. \<forall> a \<in> A. (the (m a)) = win_count_imp_code p a)"
   unfolding computewcforcands_def initmap_def
-  apply (intro WHILET_rule[where R="measure (\<lambda>(i,_). (array_length p) - i)"] refine_vcg)
-  apply auto
+  apply (intro WHILET_rule[where I="(computewcinvar A p)" 
+        and R="measure (\<lambda>(i,_). (array_length p) - i)"] refine_vcg)
+  unfolding computewcinvar_def win_count_imp_code_def
+  apply auto 
   oops (* ambitious goal *)
 
 end
